theories/program_logic/weakestpre.v
@@ -11,26 +11,26 @@ Class irisG' (Λstate : Type) (Σ : gFunctors) := IrisG {
 }.
 Notation irisG Λ Σ := (irisG' (state Λ) Σ).
 
-Definition wp_pre `{irisG Λ Σ} (p : pbit)
+Definition wp_pre `{irisG Λ Σ} (s : stuckness)
     (wp : coPset -c> expr Λ -c> (val Λ -c> iProp Σ) -c> iProp Σ) :
     coPset -c> expr Λ -c> (val Λ -c> iProp Σ) -c> iProp Σ := λ E e1 Φ,
   match to_val e1 with
   | Some v => |={E}=> Φ v
   | None => ∀ σ1,
-     state_interp σ1 ={E,∅}=∗ ⌜if p then reducible e1 σ1 else True⌝ ∗
+     state_interp σ1 ={E,∅}=∗ ⌜if s is not_stuck then reducible e1 σ1 else True⌝ ∗
      ▷ ∀ e2 σ2 efs, ⌜prim_step e1 σ1 e2 σ2 efs⌝ ={∅,E}=∗
        state_interp σ2 ∗ wp E e2 Φ ∗
        [∗ list] ef ∈ efs, wp ⊤ ef (λ _, True)
   end%I.
 
-Local Instance wp_pre_contractive `{irisG Λ Σ} p : Contractive (wp_pre p).
+Local Instance wp_pre_contractive `{irisG Λ Σ} s : Contractive (wp_pre s).
 Proof.
   rewrite /wp_pre=> n wp wp' Hwp E e1 Φ.
   repeat (f_contractive || f_equiv); apply Hwp.
 Qed.
 
-Definition wp_def `{irisG Λ Σ} p :
-  coPset → expr Λ → (val Λ → iProp Σ) → iProp Σ := fixpoint (wp_pre p).
+Definition wp_def `{irisG Λ Σ} s :
+  coPset → expr Λ → (val Λ → iProp Σ) → iProp Σ := fixpoint (wp_pre s).
 Definition wp_aux : seal (@wp_def). by eexists. Qed.
 Definition wp := unseal wp_aux.
 Definition wp_eq : @wp = @wp_def := seal_eq wp_aux.
@@ -38,44 +38,44 @@ Definition wp_eq : @wp = @wp_def := seal_eq wp_aux.
 Arguments wp {_ _ _} _ _ _%E _.
 Instance: Params (@wp) 6.
 
-Notation "'WP' e @ p ; E {{ Φ } }" := (wp p E e%E Φ)
+Notation "'WP' e @ s ; E {{ Φ } }" := (wp s E e%E Φ)
   (at level 20, e, Φ at level 200,
-   format "'[' 'WP'  e  '/' @  p ;  E  {{  Φ  } } ']'") : uPred_scope.
-Notation "'WP' e @ E {{ Φ } }" := (wp progress E e%E Φ)
+   format "'[' 'WP'  e  '/' @  s ;  E  {{  Φ  } } ']'") : uPred_scope.
+Notation "'WP' e @ E {{ Φ } }" := (wp not_stuck E e%E Φ)
   (at level 20, e, Φ at level 200,
    format "'[' 'WP'  e  '/' @  E  {{  Φ  } } ']'") : uPred_scope.
-Notation "'WP' e @ E ? {{ Φ } }" := (wp noprogress E e%E Φ)
+Notation "'WP' e @ E ? {{ Φ } }" := (wp maybe_stuck E e%E Φ)
   (at level 20, e, Φ at level 200,
    format "'[' 'WP'  e  '/' @  E  ? {{  Φ  } } ']'") : uPred_scope.
-Notation "'WP' e {{ Φ } }" := (wp progress ⊤ e%E Φ)
+Notation "'WP' e {{ Φ } }" := (wp not_stuck ⊤ e%E Φ)
   (at level 20, e, Φ at level 200,
    format "'[' 'WP'  e  '/' {{  Φ  } } ']'") : uPred_scope.
-Notation "'WP' e ? {{ Φ } }" := (wp noprogress ⊤ e%E Φ)
+Notation "'WP' e ? {{ Φ } }" := (wp maybe_stuck ⊤ e%E Φ)
   (at level 20, e, Φ at level 200,
    format "'[' 'WP'  e  '/' ? {{  Φ  } } ']'") : uPred_scope.
 
-Notation "'WP' e @ p ; E {{ v , Q } }" := (wp p E e%E (λ v, Q))
+Notation "'WP' e @ s ; E {{ v , Q } }" := (wp s E e%E (λ v, Q))
   (at level 20, e, Q at level 200,
-   format "'[' 'WP'  e  '/' @  p ;  E  {{  v ,  Q  } } ']'") : uPred_scope.
-Notation "'WP' e @ E {{ v , Q } }" := (wp progress E e%E (λ v, Q))
+   format "'[' 'WP'  e  '/' @  s ;  E  {{  v ,  Q  } } ']'") : uPred_scope.
+Notation "'WP' e @ E {{ v , Q } }" := (wp not_stuck E e%E (λ v, Q))
   (at level 20, e, Q at level 200,
    format "'[' 'WP'  e  '/' @  E  {{  v ,  Q  } } ']'") : uPred_scope.
-Notation "'WP' e @ E ? {{ v , Q } }" := (wp noprogress E e%E (λ v, Q))
+Notation "'WP' e @ E ? {{ v , Q } }" := (wp maybe_stuck E e%E (λ v, Q))
   (at level 20, e, Q at level 200,
    format "'[' 'WP'  e  '/' @  E  ? {{  v ,  Q  } } ']'") : uPred_scope.
-Notation "'WP' e {{ v , Q } }" := (wp progress ⊤ e%E (λ v, Q))
+Notation "'WP' e {{ v , Q } }" := (wp not_stuck ⊤ e%E (λ v, Q))
   (at level 20, e, Q at level 200,
    format "'[' 'WP'  e  '/' {{  v ,  Q  } } ']'") : uPred_scope.
-Notation "'WP' e ? {{ v , Q } }" := (wp noprogress ⊤ e%E (λ v, Q))
+Notation "'WP' e ? {{ v , Q } }" := (wp maybe_stuck ⊤ e%E (λ v, Q))
   (at level 20, e, Q at level 200,
    format "'[' 'WP'  e  '/' ? {{  v ,  Q  } } ']'") : uPred_scope.
 
 (* Texan triples *)
-Notation "'{{{' P } } } e @ p ; E {{{ x .. y , 'RET' pat ; Q } } }" :=
+Notation "'{{{' P } } } e @ s ; E {{{ x .. y , 'RET' pat ; Q } } }" :=
   (□ ∀ Φ,
-      P -∗ ▷ (∀ x, .. (∀ y, Q -∗ Φ pat%V) .. ) -∗ WP e @ p; E {{ Φ }})%I
+      P -∗ ▷ (∀ x, .. (∀ y, Q -∗ Φ pat%V) .. ) -∗ WP e @ s; E {{ Φ }})%I
     (at level 20, x closed binder, y closed binder,
-     format "{{{  P  } } }  e  @  p ;  E  {{{  x .. y ,  RET  pat ;  Q } } }") : uPred_scope.
+     format "{{{  P  } } }  e  @  s ;  E  {{{  x .. y ,  RET  pat ;  Q } } }") : uPred_scope.
 Notation "'{{{' P } } } e @ E {{{ x .. y , 'RET' pat ; Q } } }" :=
   (□ ∀ Φ,
       P -∗ ▷ (∀ x, .. (∀ y, Q -∗ Φ pat%V) .. ) -∗ WP e @ E {{ Φ }})%I
@@ -96,10 +96,10 @@ Notation "'{{{' P } } } e ? {{{ x .. y , 'RET' pat ; Q } } }" :=
       P -∗ ▷ (∀ x, .. (∀ y, Q -∗ Φ pat%V) .. ) -∗ WP e ?{{ Φ }})%I
     (at level 20, x closed binder, y closed binder,
      format "{{{  P  } } }  e  ? {{{  x .. y ,   RET  pat ;  Q } } }") : uPred_scope.
-Notation "'{{{' P } } } e @ p ; E {{{ 'RET' pat ; Q } } }" :=
-  (□ ∀ Φ, P -∗ ▷ (Q -∗ Φ pat%V) -∗ WP e @ p; E {{ Φ }})%I
+Notation "'{{{' P } } } e @ s ; E {{{ 'RET' pat ; Q } } }" :=
+  (□ ∀ Φ, P -∗ ▷ (Q -∗ Φ pat%V) -∗ WP e @ s; E {{ Φ }})%I
     (at level 20,
-     format "{{{  P  } } }  e  @  p ;  E  {{{  RET  pat ;  Q } } }") : uPred_scope.
+     format "{{{  P  } } }  e  @  s ;  E  {{{  RET  pat ;  Q } } }") : uPred_scope.
 Notation "'{{{' P } } } e @ E {{{ 'RET' pat ; Q } } }" :=
   (□ ∀ Φ, P -∗ ▷ (Q -∗ Φ pat%V) -∗ WP e @ E {{ Φ }})%I
     (at level 20,
@@ -117,11 +117,11 @@ Notation "'{{{' P } } } e ? {{{ 'RET' pat ; Q } } }" :=
     (at level 20,
      format "{{{  P  } } }  e  ? {{{  RET  pat ;  Q } } }") : uPred_scope.
 
-Notation "'{{{' P } } } e @ p ; E {{{ x .. y , 'RET' pat ; Q } } }" :=
+Notation "'{{{' P } } } e @ s ; E {{{ x .. y , 'RET' pat ; Q } } }" :=
   (∀ Φ : _ → uPred _,
-      P -∗ ▷ (∀ x, .. (∀ y, Q -∗ Φ pat%V) .. ) -∗ WP e @ p; E {{ Φ }})
+      P -∗ ▷ (∀ x, .. (∀ y, Q -∗ Φ pat%V) .. ) -∗ WP e @ s; E {{ Φ }})
     (at level 20, x closed binder, y closed binder,
-     format "{{{  P  } } }  e  @  p ;  E  {{{  x .. y ,  RET  pat ;  Q } } }") : C_scope.
+     format "{{{  P  } } }  e  @  s ;  E  {{{  x .. y ,  RET  pat ;  Q } } }") : C_scope.
 Notation "'{{{' P } } } e @ E {{{ x .. y , 'RET' pat ; Q } } }" :=
   (∀ Φ : _ → uPred _,
       P -∗ ▷ (∀ x, .. (∀ y, Q -∗ Φ pat%V) .. ) -∗ WP e @ E {{ Φ }})
@@ -142,10 +142,10 @@ Notation "'{{{' P } } } e ? {{{ x .. y , 'RET' pat ; Q } } }" :=
       P -∗ ▷ (∀ x, .. (∀ y, Q -∗ Φ pat%V) .. ) -∗ WP e ?{{ Φ }})
     (at level 20, x closed binder, y closed binder,
      format "{{{  P  } } }  e  ? {{{  x .. y ,  RET  pat ;  Q } } }") : C_scope.
-Notation "'{{{' P } } } e @ p ; E {{{ 'RET' pat ; Q } } }" :=
-  (∀ Φ : _ → uPred _, P -∗ ▷ (Q -∗ Φ pat%V) -∗ WP e @ p; E {{ Φ }})
+Notation "'{{{' P } } } e @ s ; E {{{ 'RET' pat ; Q } } }" :=
+  (∀ Φ : _ → uPred _, P -∗ ▷ (Q -∗ Φ pat%V) -∗ WP e @ s; E {{ Φ }})
     (at level 20,
-     format "{{{  P  } } }  e  @  p ;  E  {{{  RET  pat ;  Q } } }") : C_scope.
+     format "{{{  P  } } }  e  @  s ;  E  {{{  RET  pat ;  Q } } }") : C_scope.
 Notation "'{{{' P } } } e @ E {{{ 'RET' pat ; Q } } }" :=
   (∀ Φ : _ → uPred _, P -∗ ▷ (Q -∗ Φ pat%V) -∗ WP e @ E {{ Φ }})
     (at level 20,
@@ -165,18 +165,18 @@ Notation "'{{{' P } } } e ? {{{ 'RET' pat ; Q } } }" :=
 
 Section wp.
 Context `{irisG Λ Σ}.
-Implicit Types p : pbit.
+Implicit Types s : stuckness.
 Implicit Types P : iProp Σ.
 Implicit Types Φ : val Λ → iProp Σ.
 Implicit Types v : val Λ.
 Implicit Types e : expr Λ.
 
 (* Weakest pre *)
-Lemma wp_unfold p E e Φ : WP e @ p; E {{ Φ }} ⊣⊢ wp_pre p (wp p) E e Φ.
-Proof. rewrite wp_eq. apply (fixpoint_unfold (wp_pre p)). Qed.
+Lemma wp_unfold s E e Φ : WP e @ s; E {{ Φ }} ⊣⊢ wp_pre s (wp s) E e Φ.
+Proof. rewrite wp_eq. apply (fixpoint_unfold (wp_pre s)). Qed.
 
-Global Instance wp_ne p E e n :
-  Proper (pointwise_relation _ (dist n) ==> dist n) (@wp Λ Σ _ p E e).
+Global Instance wp_ne s E e n :
+  Proper (pointwise_relation _ (dist n) ==> dist n) (@wp Λ Σ _ s E e).
 Proof.
   revert e. induction (lt_wf n) as [n _ IH]=> e Φ Ψ HΦ.
   rewrite !wp_unfold /wp_pre.
@@ -186,19 +186,19 @@ Proof.
   do 17 (f_contractive || f_equiv). apply IH; first lia.
   intros v. eapply dist_le; eauto with omega.
 Qed.
-Global Instance wp_proper p E e :
-  Proper (pointwise_relation _ (≡) ==> (≡)) (@wp Λ Σ _ p E e).
+Global Instance wp_proper s E e :
+  Proper (pointwise_relation _ (≡) ==> (≡)) (@wp Λ Σ _ s E e).
 Proof.
   by intros Φ Φ' ?; apply equiv_dist=>n; apply wp_ne=>v; apply equiv_dist.
 Qed.
 
-Lemma wp_value' p E Φ v : Φ v ⊢ WP of_val v @ p; E {{ Φ }}.
+Lemma wp_value' s E Φ v : Φ v ⊢ WP of_val v @ s; E {{ Φ }}.
 Proof. iIntros "HΦ". rewrite wp_unfold /wp_pre to_of_val. auto. Qed.
-Lemma wp_value_inv p E Φ v : WP of_val v @ p; E {{ Φ }} ={E}=∗ Φ v.
+Lemma wp_value_inv s E Φ v : WP of_val v @ s; E {{ Φ }} ={E}=∗ Φ v.
 Proof. by rewrite wp_unfold /wp_pre to_of_val. Qed.
 
-Lemma wp_strong_mono p E1 E2 e Φ Ψ :
-  E1 ⊆ E2 → (∀ v, Φ v ={E2}=∗ Ψ v) ∗ WP e @ p; E1 {{ Φ }} ⊢ WP e @ p; E2 {{ Ψ }}.
+Lemma wp_strong_mono s E1 E2 e Φ Ψ :
+  E1 ⊆ E2 → (∀ v, Φ v ={E2}=∗ Ψ v) ∗ WP e @ s; E1 {{ Φ }} ⊢ WP e @ s; E2 {{ Ψ }}.
 Proof.
   iIntros (?) "[HΦ H]". iLöb as "IH" forall (e). rewrite !wp_unfold /wp_pre.
   destruct (to_val e) as [v|] eqn:?.
@@ -210,8 +210,8 @@ Proof.
   iMod "Hclose" as "_". by iApply ("IH" with "HΦ").
 Qed.
 
-Lemma wp_forget_progress p E e Φ :
-  WP e @ p; E {{ Φ }} ⊢ WP e @ E ?{{ Φ }}.
+Lemma wp_forget_not_stuck s E e Φ :
+  WP e @ s; E {{ Φ }} ⊢ WP e @ E ?{{ Φ }}.
 Proof.
   iIntros "H". iLöb as "IH" forall (E e Φ). rewrite !wp_unfold /wp_pre.
   destruct (to_val e) as [v|]; first iExact "H".
@@ -224,18 +224,18 @@ Proof.
   iSplitL "Hef". by iApply ("IH" with "Hef"). exact: IH. 
 Qed.
 
-Lemma fupd_wp p E e Φ : (|={E}=> WP e @ p; E {{ Φ }}) ⊢ WP e @ p; E {{ Φ }}.
+Lemma fupd_wp s E e Φ : (|={E}=> WP e @ s; E {{ Φ }}) ⊢ WP e @ s; E {{ Φ }}.
 Proof.
   rewrite wp_unfold /wp_pre. iIntros "H". destruct (to_val e) as [v|] eqn:?.
   { by iMod "H". }
   iIntros (σ1) "Hσ1". iMod "H". by iApply "H".
 Qed.
-Lemma wp_fupd p E e Φ : WP e @ p; E {{ v, |={E}=> Φ v }} ⊢ WP e @ p; E {{ Φ }}.
-Proof. iIntros "H". iApply (wp_strong_mono p E); try iFrame; auto. Qed.
+Lemma wp_fupd s E e Φ : WP e @ s; E {{ v, |={E}=> Φ v }} ⊢ WP e @ s; E {{ Φ }}.
+Proof. iIntros "H". iApply (wp_strong_mono s E); try iFrame; auto. Qed.
 
-Lemma wp_atomic' p E1 E2 e Φ :
-  StronglyAtomic e ∨ p = progress ∧ Atomic e →
-  (|={E1,E2}=> WP e @ p; E2 {{ v, |={E2,E1}=> Φ v }}) ⊢ WP e @ p; E1 {{ Φ }}.
+Lemma wp_atomic' s E1 E2 e Φ :
+  StronglyAtomic e ∨ s = not_stuck ∧ Atomic e →
+  (|={E1,E2}=> WP e @ s; E2 {{ v, |={E2,E1}=> Φ v }}) ⊢ WP e @ s; E1 {{ Φ }}.
 Proof.
   iIntros (Hatomic) "H". rewrite !wp_unfold /wp_pre.
   destruct (to_val e) as [v|].
@@ -246,34 +246,34 @@ Proof.
   - destruct (Hstrong _ _ _ _ Hstep) as [v <-%of_to_val].
     iMod ("H" with "[#]") as "($ & H & $)"; first done.
     iMod (wp_value_inv with "H") as ">H". by iApply wp_value'.
-  - destruct p; last done. iMod ("H" with "[//]") as "(Hphy & H & $)".
+  - destruct s; last done. iMod ("H" with "[//]") as "(Hphy & H & $)".
     rewrite !wp_unfold /wp_pre. destruct (to_val e2).
     + iDestruct "H" as ">> $". by iFrame.
     + iMod ("H" with "[$]") as "[H _]".
       iDestruct "H" as %(? & ? & ? & ?). by edestruct (Hweak _ _ _ _ Hstep).
 Qed.
 
-Lemma wp_step_fupd p E1 E2 e P Φ :
+Lemma wp_step_fupd s E1 E2 e P Φ :
   to_val e = None → E2 ⊆ E1 →
-  (|={E1,E2}▷=> P) -∗ WP e @ p; E2 {{ v, P ={E1}=∗ Φ v }} -∗ WP e @ p; E1 {{ Φ }}.
+  (|={E1,E2}▷=> P) -∗ WP e @ s; E2 {{ v, P ={E1}=∗ Φ v }} -∗ WP e @ s; E1 {{ Φ }}.
 Proof.
   rewrite !wp_unfold /wp_pre. iIntros (-> ?) "HR H".
   iIntros (σ1) "Hσ". iMod "HR". iMod ("H" with "[$]") as "[$ H]".
   iModIntro; iNext; iIntros (e2 σ2 efs Hstep).
   iMod ("H" $! e2 σ2 efs with "[% //]") as "($ & H & $)".
-  iMod "HR". iModIntro. iApply (wp_strong_mono p E2); first done.
+  iMod "HR". iModIntro. iApply (wp_strong_mono s E2); first done.
   iSplitR "H"; last iExact "H". iIntros (v) "H". by iApply "H".
 Qed.
 
-Lemma wp_bind K `{!LanguageCtx Λ K} p E e Φ :
-  WP e @ p; E {{ v, WP K (of_val v) @ p; E {{ Φ }} }} ⊢ WP K e @ p; E {{ Φ }}.
+Lemma wp_bind K `{!LanguageCtx Λ K} s E e Φ :
+  WP e @ s; E {{ v, WP K (of_val v) @ s; E {{ Φ }} }} ⊢ WP K e @ s; E {{ Φ }}.
 Proof.
   iIntros "H". iLöb as "IH" forall (E e Φ). rewrite wp_unfold /wp_pre.
   destruct (to_val e) as [v|] eqn:He.
   { apply of_to_val in He as <-. by iApply fupd_wp. }
   rewrite wp_unfold /wp_pre fill_not_val //.
   iIntros (σ1) "Hσ". iMod ("H" with "[$]") as "[% H]". iModIntro; iSplit.
-  { iPureIntro. destruct p; last done.
+  { iPureIntro. destruct s; last done.
     unfold reducible in *. naive_solver eauto using fill_step. }
   iNext; iIntros (e2 σ2 efs Hstep).
   destruct (fill_step_inv e σ1 e2 σ2 efs) as (e2'&->&?); auto.
@@ -281,86 +281,86 @@ Proof.
   by iApply "IH".
 Qed.
 
-Lemma wp_bind_inv K `{!LanguageCtx Λ K} p E e Φ :
-  WP K e @ p; E {{ Φ }} ⊢ WP e @ p; E {{ v, WP K (of_val v) @ p; E {{ Φ }} }}.
+Lemma wp_bind_inv K `{!LanguageCtx Λ K} s E e Φ :
+  WP K e @ s; E {{ Φ }} ⊢ WP e @ s; E {{ v, WP K (of_val v) @ s; E {{ Φ }} }}.
 Proof.
   iIntros "H". iLöb as "IH" forall (E e Φ). rewrite !wp_unfold /wp_pre.
   destruct (to_val e) as [v|] eqn:He.
   { apply of_to_val in He as <-. by rewrite !wp_unfold /wp_pre. }
   rewrite fill_not_val //.
   iIntros (σ1) "Hσ". iMod ("H" with "[$]") as "[% H]". iModIntro; iSplit.
-  { destruct p; eauto using reducible_fill. }
+  { destruct s; eauto using reducible_fill. }
   iNext; iIntros (e2 σ2 efs Hstep).
   iMod ("H" $! (K e2) σ2 efs with "[]") as "($ & H & $)"; eauto using fill_step.
   by iApply "IH".
 Qed.
 
 (** * Derived rules *)
-Lemma wp_mono p E e Φ Ψ : (∀ v, Φ v ⊢ Ψ v) → WP e @ p; E {{ Φ }} ⊢ WP e @ p; E {{ Ψ }}.
+Lemma wp_mono s E e Φ Ψ : (∀ v, Φ v ⊢ Ψ v) → WP e @ s; E {{ Φ }} ⊢ WP e @ s; E {{ Ψ }}.
 Proof.
-  iIntros (HΦ) "H"; iApply (wp_strong_mono p E E); auto.
+  iIntros (HΦ) "H"; iApply (wp_strong_mono s E E); auto.
   iIntros "{$H}" (v) "?". by iApply HΦ.
 Qed.
-Lemma wp_mask_mono p E1 E2 e Φ : E1 ⊆ E2 → WP e @ p; E1 {{ Φ }} ⊢ WP e @ p; E2 {{ Φ }}.
-Proof. iIntros (?) "H"; iApply (wp_strong_mono p E1 E2); auto. iFrame; eauto. Qed.
-Global Instance wp_mono' p E e :
-  Proper (pointwise_relation _ (⊢) ==> (⊢)) (@wp Λ Σ _ p E e).
+Lemma wp_mask_mono s E1 E2 e Φ : E1 ⊆ E2 → WP e @ s; E1 {{ Φ }} ⊢ WP e @ s; E2 {{ Φ }}.
+Proof. iIntros (?) "H"; iApply (wp_strong_mono s E1 E2); auto. iFrame; eauto. Qed.
+Global Instance wp_mono' s E e :
+  Proper (pointwise_relation _ (⊢) ==> (⊢)) (@wp Λ Σ _ s E e).
 Proof. by intros Φ Φ' ?; apply wp_mono. Qed.
 
-Lemma wp_value p E Φ e v `{!IntoVal e v} : Φ v ⊢ WP e @ p; E {{ Φ }}.
+Lemma wp_value s E Φ e v `{!IntoVal e v} : Φ v ⊢ WP e @ s; E {{ Φ }}.
 Proof. intros; rewrite -(of_to_val e v) //; by apply wp_value'. Qed.
-Lemma wp_value_fupd' p E Φ v : (|={E}=> Φ v) ⊢ WP of_val v @ p; E {{ Φ }}.
+Lemma wp_value_fupd' s E Φ v : (|={E}=> Φ v) ⊢ WP of_val v @ s; E {{ Φ }}.
 Proof. intros. by rewrite -wp_fupd -wp_value'. Qed.
-Lemma wp_value_fupd p E Φ e v `{!IntoVal e v} :
-  (|={E}=> Φ v) ⊢ WP e @ p; E {{ Φ }}.
+Lemma wp_value_fupd s E Φ e v `{!IntoVal e v} :
+  (|={E}=> Φ v) ⊢ WP e @ s; E {{ Φ }}.
 Proof. intros. rewrite -wp_fupd -wp_value //. Qed.
 
-Lemma wp_strong_atomic p E1 E2 e Φ :
+Lemma wp_strong_atomic s E1 E2 e Φ :
   StronglyAtomic e →
-  (|={E1,E2}=> WP e @ p; E2 {{ v, |={E2,E1}=> Φ v }}) ⊢ WP e @ p; E1 {{ Φ }}.
+  (|={E1,E2}=> WP e @ s; E2 {{ v, |={E2,E1}=> Φ v }}) ⊢ WP e @ s; E1 {{ Φ }}.
 Proof. by eauto using wp_atomic'. Qed.
 Lemma wp_atomic E1 E2 e Φ :
   Atomic e →
   (|={E1,E2}=> WP e @ E2 {{ v, |={E2,E1}=> Φ v }}) ⊢ WP e @ E1 {{ Φ }}.
 Proof. by eauto using wp_atomic'. Qed.
 
-Lemma wp_frame_l p E e Φ R : R ∗ WP e @ p; E {{ Φ }} ⊢ WP e @ p; E {{ v, R ∗ Φ v }}.
-Proof. iIntros "[??]". iApply (wp_strong_mono p E E _ Φ); try iFrame; eauto. Qed.
-Lemma wp_frame_r p E e Φ R : WP e @ p; E {{ Φ }} ∗ R ⊢ WP e @ p; E {{ v, Φ v ∗ R }}.
-Proof. iIntros "[??]". iApply (wp_strong_mono p E E _ Φ); try iFrame; eauto. Qed.
+Lemma wp_frame_l s E e Φ R : R ∗ WP e @ s; E {{ Φ }} ⊢ WP e @ s; E {{ v, R ∗ Φ v }}.
+Proof. iIntros "[??]". iApply (wp_strong_mono s E E _ Φ); try iFrame; eauto. Qed.
+Lemma wp_frame_r s E e Φ R : WP e @ s; E {{ Φ }} ∗ R ⊢ WP e @ s; E {{ v, Φ v ∗ R }}.
+Proof. iIntros "[??]". iApply (wp_strong_mono s E E _ Φ); try iFrame; eauto. Qed.
 
-Lemma wp_frame_step_l p E1 E2 e Φ R :
+Lemma wp_frame_step_l s E1 E2 e Φ R :
   to_val e = None → E2 ⊆ E1 →
-  (|={E1,E2}▷=> R) ∗ WP e @ p; E2 {{ Φ }} ⊢ WP e @ p; E1 {{ v, R ∗ Φ v }}.
+  (|={E1,E2}▷=> R) ∗ WP e @ s; E2 {{ Φ }} ⊢ WP e @ s; E1 {{ v, R ∗ Φ v }}.
 Proof.
   iIntros (??) "[Hu Hwp]". iApply (wp_step_fupd with "Hu"); try done.
   iApply (wp_mono with "Hwp"). by iIntros (?) "$$".
 Qed.
-Lemma wp_frame_step_r p E1 E2 e Φ R :
+Lemma wp_frame_step_r s E1 E2 e Φ R :
   to_val e = None → E2 ⊆ E1 →
-  WP e @ p; E2 {{ Φ }} ∗ (|={E1,E2}▷=> R) ⊢ WP e @ p; E1 {{ v, Φ v ∗ R }}.
+  WP e @ s; E2 {{ Φ }} ∗ (|={E1,E2}▷=> R) ⊢ WP e @ s; E1 {{ v, Φ v ∗ R }}.
 Proof.
   rewrite [(WP _ @ _; _ {{ _ }} ∗ _)%I]comm; setoid_rewrite (comm _ _ R).
   apply wp_frame_step_l.
 Qed.
-Lemma wp_frame_step_l' p E e Φ R :
-  to_val e = None → ▷ R ∗ WP e @ p; E {{ Φ }} ⊢ WP e @ p; E {{ v, R ∗ Φ v }}.
-Proof. iIntros (?) "[??]". iApply (wp_frame_step_l p E E); try iFrame; eauto. Qed.
-Lemma wp_frame_step_r' p E e Φ R :
-  to_val e = None → WP e @ p; E {{ Φ }} ∗ ▷ R ⊢ WP e @ p; E {{ v, Φ v ∗ R }}.
-Proof. iIntros (?) "[??]". iApply (wp_frame_step_r p E E); try iFrame; eauto. Qed.
+Lemma wp_frame_step_l' s E e Φ R :
+  to_val e = None → ▷ R ∗ WP e @ s; E {{ Φ }} ⊢ WP e @ s; E {{ v, R ∗ Φ v }}.
+Proof. iIntros (?) "[??]". iApply (wp_frame_step_l s E E); try iFrame; eauto. Qed.
+Lemma wp_frame_step_r' s E e Φ R :
+  to_val e = None → WP e @ s; E {{ Φ }} ∗ ▷ R ⊢ WP e @ s; E {{ v, Φ v ∗ R }}.
+Proof. iIntros (?) "[??]". iApply (wp_frame_step_r s E E); try iFrame; eauto. Qed.
 
-Lemma wp_wand p E e Φ Ψ :
-  WP e @ p; E {{ Φ }} -∗ (∀ v, Φ v -∗ Ψ v) -∗ WP e @ p; E {{ Ψ }}.
+Lemma wp_wand s E e Φ Ψ :
+  WP e @ s; E {{ Φ }} -∗ (∀ v, Φ v -∗ Ψ v) -∗ WP e @ s; E {{ Ψ }}.
 Proof.
-  iIntros "Hwp H". iApply (wp_strong_mono p E); auto.
+  iIntros "Hwp H". iApply (wp_strong_mono s E); auto.
   iIntros "{$Hwp}" (?) "?". by iApply "H".
 Qed.
-Lemma wp_wand_l p E e Φ Ψ :
-  (∀ v, Φ v -∗ Ψ v) ∗ WP e @ p; E {{ Φ }} ⊢ WP e @ p; E {{ Ψ }}.
+Lemma wp_wand_l s E e Φ Ψ :
+  (∀ v, Φ v -∗ Ψ v) ∗ WP e @ s; E {{ Φ }} ⊢ WP e @ s; E {{ Ψ }}.
 Proof. iIntros "[H Hwp]". iApply (wp_wand with "Hwp H"). Qed.
-Lemma wp_wand_r p E e Φ Ψ :
-  WP e @ p; E {{ Φ }} ∗ (∀ v, Φ v -∗ Ψ v) ⊢ WP e @ p; E {{ Ψ }}.
+Lemma wp_wand_r s E e Φ Ψ :
+  WP e @ s; E {{ Φ }} ∗ (∀ v, Φ v -∗ Ψ v) ⊢ WP e @ s; E {{ Ψ }}.
 Proof. iIntros "[Hwp H]". iApply (wp_wand with "Hwp H"). Qed.
 End wp.
 
@@ -370,26 +370,26 @@ Section proofmode_classes.
   Implicit Types P Q : iProp Σ.
   Implicit Types Φ : val Λ → iProp Σ.
 
-  Global Instance frame_wp p p' E e R Φ Ψ :
-    (∀ v, Frame p' R (Φ v) (Ψ v)) → Frame p' R (WP e @ p; E {{ Φ }}) (WP e @ p; E {{ Ψ }}).
+  Global Instance frame_wp p s E e R Φ Ψ :
+    (∀ v, Frame p R (Φ v) (Ψ v)) → Frame p R (WP e @ s; E {{ Φ }}) (WP e @ s; E {{ Ψ }}).
   Proof. rewrite /Frame=> HR. rewrite wp_frame_l. apply wp_mono, HR. Qed.
 
-  Global Instance is_except_0_wp p E e Φ : IsExcept0 (WP e @ p; E {{ Φ }}).
+  Global Instance is_except_0_wp s E e Φ : IsExcept0 (WP e @ s; E {{ Φ }}).
   Proof. by rewrite /IsExcept0 -{2}fupd_wp -except_0_fupd -fupd_intro. Qed.
 
-  Global Instance elim_modal_bupd_wp p E e P Φ :
-    ElimModal (|==> P) P (WP e @ p; E {{ Φ }}) (WP e @ p; E {{ Φ }}).
+  Global Instance elim_modal_bupd_wp s E e P Φ :
+    ElimModal (|==> P) P (WP e @ s; E {{ Φ }}) (WP e @ s; E {{ Φ }}).
   Proof. by rewrite /ElimModal (bupd_fupd E) fupd_frame_r wand_elim_r fupd_wp. Qed.
 
-  Global Instance elim_modal_fupd_wp p E e P Φ :
-    ElimModal (|={E}=> P) P (WP e @ p; E {{ Φ }}) (WP e @ p; E {{ Φ }}).
+  Global Instance elim_modal_fupd_wp s E e P Φ :
+    ElimModal (|={E}=> P) P (WP e @ s; E {{ Φ }}) (WP e @ s; E {{ Φ }}).
   Proof. by rewrite /ElimModal fupd_frame_r wand_elim_r fupd_wp. Qed.
 
   (* lower precedence, if possible, it should persistently pick elim_upd_fupd_wp *)
   Global Instance elim_modal_fupd_wp_strong_atomic E1 E2 e P Φ :
     StronglyAtomic e →
     ElimModal (|={E1,E2}=> P) P
-            (WP e @ p; E1 {{ Φ }}) (WP e @ p; E2 {{ v, |={E2,E1}=> Φ v }})%I | 100.
+            (WP e @ s; E1 {{ Φ }}) (WP e @ s; E2 {{ v, |={E2,E1}=> Φ v }})%I | 100.
   Proof. intros. by rewrite /ElimModal fupd_frame_r wand_elim_r wp_strong_atomic. Qed.
 
   (* lower precedence than elim_modal_fupd_wp_strong_atomic (for no good reason) *)
