theories/program_logic/ectx_lifting.v
@@ -6,7 +6,7 @@ Set Default Proof Using "Type".
 Section wp.
 Context {expr val ectx state} {Λ : EctxLanguage expr val ectx state}.
 Context `{irisG (ectx_lang expr) Σ} {Hinh : Inhabited state}.
-Implicit Types p : pbit.
+Implicit Types s : stuckness.
 Implicit Types P : iProp Σ.
 Implicit Types Φ : val → iProp Σ.
 Implicit Types v : val.
@@ -15,27 +15,27 @@ Hint Resolve head_prim_reducible head_reducible_prim_step.
 Hint Resolve (reducible_not_val _ inhabitant).
 Hint Resolve progressive_head_progressive.
 
-Lemma wp_ectx_bind {p E e} K Φ :
-  WP e @ p; E {{ v, WP fill K (of_val v) @ p; E {{ Φ }} }}
-  ⊢ WP fill K e @ p; E {{ Φ }}.
+Lemma wp_ectx_bind {s E e} K Φ :
+  WP e @ s; E {{ v, WP fill K (of_val v) @ s; E {{ Φ }} }}
+  ⊢ WP fill K e @ s; E {{ Φ }}.
 Proof. apply: weakestpre.wp_bind. Qed.
 
-Lemma wp_ectx_bind_inv {p E Φ} K e :
-  WP fill K e @ p; E {{ Φ }}
-  ⊢ WP e @ p; E {{ v, WP fill K (of_val v) @ p; E {{ Φ }} }}.
+Lemma wp_ectx_bind_inv {s E Φ} K e :
+  WP fill K e @ s; E {{ Φ }}
+  ⊢ WP e @ s; E {{ v, WP fill K (of_val v) @ s; E {{ Φ }} }}.
 Proof. apply: weakestpre.wp_bind_inv. Qed.
 
-Lemma wp_lift_head_step {p E Φ} e1 :
+Lemma wp_lift_head_step {s E Φ} e1 :
   to_val e1 = None →
   (∀ σ1, state_interp σ1 ={E,∅}=∗
     ⌜head_reducible e1 σ1⌝ ∗
     ▷ ∀ e2 σ2 efs, ⌜head_step e1 σ1 e2 σ2 efs⌝ ={∅,E}=∗
-      state_interp σ2 ∗ WP e2 @ p; E {{ Φ }} ∗ [∗ list] ef ∈ efs, WP ef @ p; ⊤ {{ _, True }})
-  ⊢ WP e1 @ p; E {{ Φ }}.
+      state_interp σ2 ∗ WP e2 @ s; E {{ Φ }} ∗ [∗ list] ef ∈ efs, WP ef @ s; ⊤ {{ _, True }})
+  ⊢ WP e1 @ s; E {{ Φ }}.
 Proof.
   iIntros (?) "H". iApply wp_lift_step=>//. iIntros (σ1) "Hσ".
   iMod ("H" with "Hσ") as "[% H]"; iModIntro.
-  iSplit; first by destruct p; eauto. iNext. iIntros (e2 σ2 efs) "%".
+  iSplit; first by destruct s; eauto. iNext. iIntros (e2 σ2 efs) "%".
   iApply "H"; eauto.
 Qed.
 
@@ -48,15 +48,15 @@ Proof.
   iIntros (σ) "Hσ". iMod ("H" with "Hσ") as "%". by auto. 
 Qed.
 
-Lemma wp_lift_pure_head_step {p E E' Φ} e1 :
+Lemma wp_lift_pure_head_step {s E E' Φ} e1 :
   (∀ σ1, head_reducible e1 σ1) →
   (∀ σ1 e2 σ2 efs, head_step e1 σ1 e2 σ2 efs → σ1 = σ2) →
   (|={E,E'}▷=> ∀ e2 efs σ, ⌜head_step e1 σ e2 σ efs⌝ →
-    WP e2 @ p; E {{ Φ }} ∗ [∗ list] ef ∈ efs, WP ef @ p; ⊤ {{ _, True }})
-  ⊢ WP e1 @ p; E {{ Φ }}.
+    WP e2 @ s; E {{ Φ }} ∗ [∗ list] ef ∈ efs, WP ef @ s; ⊤ {{ _, True }})
+  ⊢ WP e1 @ s; E {{ Φ }}.
 Proof using Hinh.
   iIntros (??) "H". iApply wp_lift_pure_step; eauto.
-  { by destruct p; auto. }
+  { by destruct s; auto. }
   iApply (step_fupd_wand with "H"); iIntros "H".
   iIntros (????). iApply "H"; eauto.
 Qed.
@@ -72,28 +72,28 @@ Proof using Hinh.
   move=>[] K [] e1 [] Hfill [] e2 [] σ2 [] efs /= Hstep. exact: Hnstep.
 Qed.
 
-Lemma wp_lift_atomic_head_step {p E Φ} e1 :
+Lemma wp_lift_atomic_head_step {s E Φ} e1 :
   to_val e1 = None →
   (∀ σ1, state_interp σ1 ={E}=∗
     ⌜head_reducible e1 σ1⌝ ∗
     ▷ ∀ e2 σ2 efs, ⌜head_step e1 σ1 e2 σ2 efs⌝ ={E}=∗
       state_interp σ2 ∗
-      default False (to_val e2) Φ ∗ [∗ list] ef ∈ efs, WP ef @ p; ⊤ {{ _, True }})
-  ⊢ WP e1 @ p; E {{ Φ }}.
+      default False (to_val e2) Φ ∗ [∗ list] ef ∈ efs, WP ef @ s; ⊤ {{ _, True }})
+  ⊢ WP e1 @ s; E {{ Φ }}.
 Proof.
   iIntros (?) "H". iApply wp_lift_atomic_step; eauto.
   iIntros (σ1) "Hσ1". iMod ("H" with "Hσ1") as "[% H]"; iModIntro.
-  iSplit; first by destruct p; auto. iNext. iIntros (e2 σ2 efs) "%".
+  iSplit; first by destruct s; auto. iNext. iIntros (e2 σ2 efs) "%".
   iApply "H"; auto.
 Qed.
 
-Lemma wp_lift_atomic_head_step_no_fork {p E Φ} e1 :
+Lemma wp_lift_atomic_head_step_no_fork {s E Φ} e1 :
   to_val e1 = None →
   (∀ σ1, state_interp σ1 ={E}=∗
     ⌜head_reducible e1 σ1⌝ ∗
     ▷ ∀ e2 σ2 efs, ⌜head_step e1 σ1 e2 σ2 efs⌝ ={E}=∗
       ⌜efs = []⌝ ∗ state_interp σ2 ∗ default False (to_val e2) Φ)
-  ⊢ WP e1 @ p; E {{ Φ }}.
+  ⊢ WP e1 @ s; E {{ Φ }}.
 Proof.
   iIntros (?) "H". iApply wp_lift_atomic_head_step; eauto.
   iIntros (σ1) "Hσ1". iMod ("H" $! σ1 with "Hσ1") as "[$ H]"; iModIntro.
@@ -101,29 +101,29 @@ Proof.
   iMod ("H" $! v2 σ2 efs with "[# //]") as "(% & $ & $)"; subst; auto.
 Qed.
 
-Lemma wp_lift_pure_det_head_step {p E E' Φ} e1 e2 efs :
+Lemma wp_lift_pure_det_head_step {s E E' Φ} e1 e2 efs :
   (∀ σ1, head_reducible e1 σ1) →
   (∀ σ1 e2' σ2 efs',
     head_step e1 σ1 e2' σ2 efs' → σ1 = σ2 ∧ e2 = e2' ∧ efs = efs') →
-  (|={E,E'}▷=> WP e2 @ p; E {{ Φ }} ∗ [∗ list] ef ∈ efs, WP ef @ p; ⊤ {{ _, True }})
-  ⊢ WP e1 @ p; E {{ Φ }}.
+  (|={E,E'}▷=> WP e2 @ s; E {{ Φ }} ∗ [∗ list] ef ∈ efs, WP ef @ s; ⊤ {{ _, True }})
+  ⊢ WP e1 @ s; E {{ Φ }}.
 Proof using Hinh.
   intros. rewrite -(wp_lift_pure_det_step e1 e2 efs); eauto.
-  destruct p; by auto.
+  destruct s; by auto.
 Qed.
 
-Lemma wp_lift_pure_det_head_step_no_fork {p E E' Φ} e1 e2 :
+Lemma wp_lift_pure_det_head_step_no_fork {s E E' Φ} e1 e2 :
   to_val e1 = None →
   (∀ σ1, head_reducible e1 σ1) →
   (∀ σ1 e2' σ2 efs',
     head_step e1 σ1 e2' σ2 efs' → σ1 = σ2 ∧ e2 = e2' ∧ [] = efs') →
-  (|={E,E'}▷=> WP e2 @ p; E {{ Φ }}) ⊢ WP e1 @ p; E {{ Φ }}.
+  (|={E,E'}▷=> WP e2 @ s; E {{ Φ }}) ⊢ WP e1 @ s; E {{ Φ }}.
 Proof using Hinh.
   intros. rewrite -(wp_lift_pure_det_step e1 e2 []) /= ?right_id; eauto.
-  destruct p; by auto.
+  destruct s; by auto.
 Qed.
 
-Lemma wp_lift_pure_det_head_step_no_fork' {p E Φ} e1 e2 :
+Lemma wp_lift_pure_det_head_step_no_fork' {s E Φ} e1 e2 :
   to_val e1 = None →
   (∀ σ1, head_reducible e1 σ1) →
   (∀ σ1 e2' σ2 efs',
