theories/program_logic/ownp.v
@@ -39,9 +39,9 @@ Instance: Params (@ownP) 3.
 
 
 (* Adequacy *)
-Theorem ownP_adequacy Σ `{ownPPreG Λ Σ} p e σ φ :
-  (∀ `{ownPG Λ Σ}, ownP σ ⊢ WP e @ p; ⊤ {{ v, ⌜φ v⌝ }}) →
-  adequate p e σ φ.
+Theorem ownP_adequacy Σ `{ownPPreG Λ Σ} s e σ φ :
+  (∀ `{ownPG Λ Σ}, ownP σ ⊢ WP e @ s; ⊤ {{ v, ⌜φ v⌝ }}) →
+  adequate s e σ φ.
 Proof.
   intros Hwp. apply (wp_adequacy Σ _).
   iIntros (?) "". iMod (own_alloc (● (Excl' (σ : leibnizC _)) ⋅ ◯ (Excl' σ)))
@@ -50,13 +50,13 @@ Proof.
   iApply (Hwp (OwnPG _ _ _ _ γσ)). by rewrite /ownP.
 Qed.
 
-Theorem ownP_invariance Σ `{ownPPreG Λ Σ} p e σ1 t2 σ2 φ :
+Theorem ownP_invariance Σ `{ownPPreG Λ Σ} s e σ1 t2 σ2 φ :
   (∀ `{ownPG Λ Σ},
-    ownP σ1 ={⊤}=∗ WP e @ p; ⊤ {{ _, True }} ∗ |={⊤,∅}=> ∃ σ', ownP σ' ∧ ⌜φ σ'⌝) →
+    ownP σ1 ={⊤}=∗ WP e @ s; ⊤ {{ _, True }} ∗ |={⊤,∅}=> ∃ σ', ownP σ' ∧ ⌜φ σ'⌝) →
   rtc step ([e], σ1) (t2, σ2) →
   φ σ2.
 Proof.
-  intros Hwp Hsteps. eapply (wp_invariance Σ Λ p e σ1 t2 σ2 _)=> //.
+  intros Hwp Hsteps. eapply (wp_invariance Σ Λ s e σ1 t2 σ2 _)=> //.
   iIntros (?) "". iMod (own_alloc (● (Excl' (σ1 : leibnizC _)) ⋅ ◯ (Excl' σ1)))
     as (γσ) "[Hσ Hσf]"; first done.
   iExists (λ σ, own γσ (● (Excl' (σ:leibnizC _)))). iFrame "Hσ".
@@ -70,7 +70,7 @@ Qed.
 (** Lifting *)
 Section lifting.
   Context `{ownPG Λ Σ}.
-  Implicit Types p : pbit.
+  Implicit Types s : stuckness.
   Implicit Types e : expr Λ.
   Implicit Types Φ : val Λ → iProp Σ.
 
@@ -85,12 +85,12 @@ Section lifting.
   Global Instance ownP_timeless σ : Timeless (@ownP (state Λ) Σ _ σ).
   Proof. rewrite /ownP; apply _. Qed.
 
-  Lemma ownP_lift_step p E Φ e1 :
+  Lemma ownP_lift_step s E Φ e1 :
     to_val e1 = None →
-    (|={E,∅}=> ∃ σ1, ⌜if p then reducible e1 σ1 else True⌝ ∗ ▷ ownP σ1 ∗
+    (|={E,∅}=> ∃ σ1, ⌜if s is not_stuck then reducible e1 σ1 else True⌝ ∗ ▷ ownP σ1 ∗
       ▷ ∀ e2 σ2 efs, ⌜prim_step e1 σ1 e2 σ2 efs⌝ -∗ ownP σ2
-            ={∅,E}=∗ WP e2 @ p; E {{ Φ }} ∗ [∗ list] ef ∈ efs, WP ef @ p; ⊤ {{ _, True }})
-    ⊢ WP e1 @ p; E {{ Φ }}.
+            ={∅,E}=∗ WP e2 @ s; E {{ Φ }} ∗ [∗ list] ef ∈ efs, WP ef @ s; ⊤ {{ _, True }})
+    ⊢ WP e1 @ s; E {{ Φ }}.
   Proof.
     iIntros (?) "H". iApply wp_lift_step; first done.
     iIntros (σ1) "Hσ"; iMod "H" as (σ1') "(% & >Hσf & H)".
@@ -115,79 +115,79 @@ Section lifting.
       by iDestruct (ownP_eq with "Hσ Hσf") as %->.
   Qed.
 
-  Lemma ownP_lift_pure_step p E Φ e1 :
+  Lemma ownP_lift_pure_step s E Φ e1 :
     to_val e1 = None →
-    (∀ σ1, if p then reducible e1 σ1 else True) →
+    (∀ σ1, if s is not_stuck then reducible e1 σ1 else True) →
     (∀ σ1 e2 σ2 efs, prim_step e1 σ1 e2 σ2 efs → σ1 = σ2) →
     (▷ ∀ e2 efs σ, ⌜prim_step e1 σ e2 σ efs⌝ →
-      WP e2 @ p; E {{ Φ }} ∗ [∗ list] ef ∈ efs, WP ef @ p; ⊤ {{ _, True }})
-    ⊢ WP e1 @ p; E {{ Φ }}.
+      WP e2 @ s; E {{ Φ }} ∗ [∗ list] ef ∈ efs, WP ef @ s; ⊤ {{ _, True }})
+    ⊢ WP e1 @ s; E {{ Φ }}.
   Proof.
     iIntros (? Hsafe Hstep) "H"; iApply wp_lift_step; first done.
     iIntros (σ1) "Hσ". iMod (fupd_intro_mask' E ∅) as "Hclose"; first set_solver.
-    iModIntro; iSplit; [by destruct p|]; iNext; iIntros (e2 σ2 efs ?).
+    iModIntro; iSplit; [by destruct s|]; iNext; iIntros (e2 σ2 efs ?).
     destruct (Hstep σ1 e2 σ2 efs); auto; subst.
     by iMod "Hclose"; iModIntro; iFrame; iApply "H".
   Qed.
 
   (** Derived lifting lemmas. *)
-  Lemma ownP_lift_atomic_step {p E Φ} e1 σ1 :
+  Lemma ownP_lift_atomic_step {s E Φ} e1 σ1 :
     to_val e1 = None →
-    (if p then reducible e1 σ1 else True) →
+    (if s is not_stuck then reducible e1 σ1 else True) →
     (▷ ownP σ1 ∗ ▷ ∀ e2 σ2 efs, ⌜prim_step e1 σ1 e2 σ2 efs⌝ -∗ ownP σ2 -∗
-      default False (to_val e2) Φ ∗ [∗ list] ef ∈ efs, WP ef @ p; ⊤ {{ _, True }})
-    ⊢ WP e1 @ p; E {{ Φ }}.
+      default False (to_val e2) Φ ∗ [∗ list] ef ∈ efs, WP ef @ s; ⊤ {{ _, True }})
+    ⊢ WP e1 @ s; E {{ Φ }}.
   Proof.
     iIntros (??) "[Hσ H]"; iApply ownP_lift_step; first done.
     iMod (fupd_intro_mask' E ∅) as "Hclose"; first set_solver.
-    iModIntro; iExists σ1; iFrame; iSplit; first by destruct p.
+    iModIntro; iExists σ1; iFrame; iSplit; first by destruct s.
     iNext; iIntros (e2 σ2 efs) "% Hσ".
     iDestruct ("H" $! e2 σ2 efs with "[] [Hσ]") as "[HΦ $]"; [by eauto..|].
     destruct (to_val e2) eqn:?; last by iExFalso.
     by iMod "Hclose"; iApply wp_value; auto using to_of_val.
   Qed.
 
-  Lemma ownP_lift_atomic_det_step {p E Φ e1} σ1 v2 σ2 efs :
+  Lemma ownP_lift_atomic_det_step {s E Φ e1} σ1 v2 σ2 efs :
     to_val e1 = None →
-    (if p then reducible e1 σ1 else True) →
+    (if s is not_stuck then reducible e1 σ1 else True) →
     (∀ e2' σ2' efs', prim_step e1 σ1 e2' σ2' efs' →
                      σ2 = σ2' ∧ to_val e2' = Some v2 ∧ efs = efs') →
     ▷ ownP σ1 ∗ ▷ (ownP σ2 -∗
-      Φ v2 ∗ [∗ list] ef ∈ efs, WP ef @ p; ⊤ {{ _, True }})
-    ⊢ WP e1 @ p; E {{ Φ }}.
+      Φ v2 ∗ [∗ list] ef ∈ efs, WP ef @ s; ⊤ {{ _, True }})
+    ⊢ WP e1 @ s; E {{ Φ }}.
   Proof.
     iIntros (?? Hdet) "[Hσ1 Hσ2]"; iApply ownP_lift_atomic_step; try done.
     iFrame; iNext; iIntros (e2' σ2' efs') "% Hσ2'".
     edestruct Hdet as (->&Hval&->). done. by rewrite Hval; iApply "Hσ2".
   Qed.
 
-  Lemma ownP_lift_atomic_det_step_no_fork {p E e1} σ1 v2 σ2 :
+  Lemma ownP_lift_atomic_det_step_no_fork {s E e1} σ1 v2 σ2 :
     to_val e1 = None →
-    (if p then reducible e1 σ1 else True) →
+    (if s is not_stuck then reducible e1 σ1 else True) →
     (∀ e2' σ2' efs', prim_step e1 σ1 e2' σ2' efs' →
       σ2 = σ2' ∧ to_val e2' = Some v2 ∧ [] = efs') →
-    {{{ ▷ ownP σ1 }}} e1 @ p; E {{{ RET v2; ownP σ2 }}}.
+    {{{ ▷ ownP σ1 }}} e1 @ s; E {{{ RET v2; ownP σ2 }}}.
   Proof.
     intros. rewrite -(ownP_lift_atomic_det_step σ1 v2 σ2 []); [|done..].
     rewrite big_sepL_nil right_id. by apply uPred.wand_intro_r.
   Qed.
 
-  Lemma ownP_lift_pure_det_step {p E Φ} e1 e2 efs :
+  Lemma ownP_lift_pure_det_step {s E Φ} e1 e2 efs :
     to_val e1 = None →
-    (∀ σ1, if p then reducible e1 σ1 else True) →
+    (∀ σ1, if s is not_stuck then reducible e1 σ1 else True) →
     (∀ σ1 e2' σ2 efs', prim_step e1 σ1 e2' σ2 efs' → σ1 = σ2 ∧ e2 = e2' ∧ efs = efs')→
-    ▷ (WP e2 @ p; E {{ Φ }} ∗ [∗ list] ef ∈ efs, WP ef @ p; ⊤{{ _, True }})
-    ⊢ WP e1 @ p; E {{ Φ }}.
+    ▷ (WP e2 @ s; E {{ Φ }} ∗ [∗ list] ef ∈ efs, WP ef @ s; ⊤{{ _, True }})
+    ⊢ WP e1 @ s; E {{ Φ }}.
   Proof.
     iIntros (?? Hpuredet) "?"; iApply ownP_lift_pure_step=>//.
     by apply Hpuredet. by iNext; iIntros (e' efs' σ (_&->&->)%Hpuredet).
   Qed.
 
-  Lemma ownP_lift_pure_det_step_no_fork `{Inhabited (state Λ)} {p E Φ} e1 e2 :
+  Lemma ownP_lift_pure_det_step_no_fork `{Inhabited (state Λ)} {s E Φ} e1 e2 :
     to_val e1 = None →
-    (∀ σ1, if p then reducible e1 σ1 else True) →
+    (∀ σ1, if s is not_stuck then reducible e1 σ1 else True) →
     (∀ σ1 e2' σ2 efs', prim_step e1 σ1 e2' σ2 efs' → σ1 = σ2 ∧ e2 = e2' ∧ [] = efs') →
-    ▷ WP e2 @ p; E {{ Φ }} ⊢ WP e1 @ p; E {{ Φ }}.
+    ▷ WP e2 @ s; E {{ Φ }} ⊢ WP e1 @ s; E {{ Φ }}.
   Proof.
     intros. rewrite -(wp_lift_pure_det_step e1 e2 []) ?big_sepL_nil ?right_id; eauto.
   Qed.
@@ -197,23 +197,23 @@ Section ectx_lifting.
   Import ectx_language.
   Context {expr val ectx state} {Λ : EctxLanguage expr val ectx state}.
   Context `{ownPG (ectx_lang expr) Σ} {Hinh : Inhabited state}.
-  Implicit Types p : pbit.
+  Implicit Types s : stuckness.
   Implicit Types Φ : val → iProp Σ.
   Implicit Types e : expr.
   Hint Resolve head_prim_reducible head_reducible_prim_step.
   Hint Resolve (reducible_not_val _ inhabitant).
   Hint Resolve progressive_head_progressive.
 
-  Lemma ownP_lift_head_step p E Φ e1 :
+  Lemma ownP_lift_head_step s E Φ e1 :
     to_val e1 = None →
     (|={E,∅}=> ∃ σ1, ⌜head_reducible e1 σ1⌝ ∗ ▷ ownP σ1 ∗
       ▷ ∀ e2 σ2 efs, ⌜head_step e1 σ1 e2 σ2 efs⌝ -∗ ownP σ2
-            ={∅,E}=∗ WP e2 @ p; E {{ Φ }} ∗ [∗ list] ef ∈ efs, WP ef @ p; ⊤ {{ _, True }})
-    ⊢ WP e1 @ p; E {{ Φ }}.
+            ={∅,E}=∗ WP e2 @ s; E {{ Φ }} ∗ [∗ list] ef ∈ efs, WP ef @ s; ⊤ {{ _, True }})
+    ⊢ WP e1 @ s; E {{ Φ }}.
   Proof.
     iIntros (?) "H". iApply ownP_lift_step; first done.
     iMod "H" as (σ1 ?) "[Hσ1 Hwp]". iModIntro. iExists σ1.
-    iSplit; first by destruct p; eauto. iFrame. iNext. iIntros (e2 σ2 efs) "% ?".
+    iSplit; first by destruct s; eauto. iFrame. iNext. iIntros (e2 σ2 efs) "% ?".
     iApply ("Hwp" with "[]"); eauto.
   Qed.
 
@@ -225,72 +225,72 @@ Section ectx_lifting.
     iModIntro. iExists σ. iFrame "Hσ". by eauto.
   Qed.
 
-  Lemma ownP_lift_pure_head_step p E Φ e1 :
+  Lemma ownP_lift_pure_head_step s E Φ e1 :
     to_val e1 = None →
     (∀ σ1, head_reducible e1 σ1) →
     (∀ σ1 e2 σ2 efs, head_step e1 σ1 e2 σ2 efs → σ1 = σ2) →
     (▷ ∀ e2 efs σ, ⌜head_step e1 σ e2 σ efs⌝ →
-      WP e2 @ p; E {{ Φ }} ∗ [∗ list] ef ∈ efs, WP ef @ p; ⊤ {{ _, True }})
-    ⊢ WP e1 @ p; E {{ Φ }}.
+      WP e2 @ s; E {{ Φ }} ∗ [∗ list] ef ∈ efs, WP ef @ s; ⊤ {{ _, True }})
+    ⊢ WP e1 @ s; E {{ Φ }}.
   Proof using Hinh.
     iIntros (???) "H".  iApply ownP_lift_pure_step; eauto.
-    { by destruct p; auto. }
+    { by destruct s; auto. }
     iNext. iIntros (????). iApply "H"; eauto.
   Qed.
 
-  Lemma ownP_lift_atomic_head_step {p E Φ} e1 σ1 :
+  Lemma ownP_lift_atomic_head_step {s E Φ} e1 σ1 :
     to_val e1 = None →
     head_reducible e1 σ1 →
     ▷ ownP σ1 ∗ ▷ (∀ e2 σ2 efs,
     ⌜head_step e1 σ1 e2 σ2 efs⌝ -∗ ownP σ2 -∗
-      default False (to_val e2) Φ ∗ [∗ list] ef ∈ efs, WP ef @ p; ⊤ {{ _, True }})
-    ⊢ WP e1 @ p; E {{ Φ }}.
+      default False (to_val e2) Φ ∗ [∗ list] ef ∈ efs, WP ef @ s; ⊤ {{ _, True }})
+    ⊢ WP e1 @ s; E {{ Φ }}.
   Proof.
     iIntros (??) "[? H]". iApply ownP_lift_atomic_step; eauto.
-    { by destruct p; eauto. }
+    { by destruct s; eauto. }
     iFrame. iNext. iIntros (???) "% ?". iApply ("H" with "[]"); eauto.
   Qed.
 
-  Lemma ownP_lift_atomic_det_head_step {p E Φ e1} σ1 v2 σ2 efs :
+  Lemma ownP_lift_atomic_det_head_step {s E Φ e1} σ1 v2 σ2 efs :
     to_val e1 = None →
     head_reducible e1 σ1 →
     (∀ e2' σ2' efs', head_step e1 σ1 e2' σ2' efs' →
       σ2 = σ2' ∧ to_val e2' = Some v2 ∧ efs = efs') →
-    ▷ ownP σ1 ∗ ▷ (ownP σ2 -∗ Φ v2 ∗ [∗ list] ef ∈ efs, WP ef @ p; ⊤ {{ _, True }})
-    ⊢ WP e1 @ p; E {{ Φ }}.
+    ▷ ownP σ1 ∗ ▷ (ownP σ2 -∗ Φ v2 ∗ [∗ list] ef ∈ efs, WP ef @ s; ⊤ {{ _, True }})
+    ⊢ WP e1 @ s; E {{ Φ }}.
   Proof.
-    by destruct p; eauto 10 using ownP_lift_atomic_det_step.
+    by destruct s; eauto 10 using ownP_lift_atomic_det_step.
   Qed.
 
-  Lemma ownP_lift_atomic_det_head_step_no_fork {p E e1} σ1 v2 σ2 :
+  Lemma ownP_lift_atomic_det_head_step_no_fork {s E e1} σ1 v2 σ2 :
     to_val e1 = None →
     head_reducible e1 σ1 →
     (∀ e2' σ2' efs', head_step e1 σ1 e2' σ2' efs' →
       σ2 = σ2' ∧ to_val e2' = Some v2 ∧ [] = efs') →
-    {{{ ▷ ownP σ1 }}} e1 @ p; E {{{ RET v2; ownP σ2 }}}.
+    {{{ ▷ ownP σ1 }}} e1 @ s; E {{{ RET v2; ownP σ2 }}}.
   Proof.
     intros ???; apply ownP_lift_atomic_det_step_no_fork; eauto.
-    by destruct p; eauto.
+    by destruct s; eauto.
   Qed.
 
-  Lemma ownP_lift_pure_det_head_step {p E Φ} e1 e2 efs :
+  Lemma ownP_lift_pure_det_head_step {s E Φ} e1 e2 efs :
     to_val e1 = None →
     (∀ σ1, head_reducible e1 σ1) →
     (∀ σ1 e2' σ2 efs', head_step e1 σ1 e2' σ2 efs' → σ1 = σ2 ∧ e2 = e2' ∧ efs = efs') →
-    ▷ (WP e2 @ p; E {{ Φ }} ∗ [∗ list] ef ∈ efs, WP ef @ p; ⊤ {{ _, True }})
-    ⊢ WP e1 @ p; E {{ Φ }}.
+    ▷ (WP e2 @ s; E {{ Φ }} ∗ [∗ list] ef ∈ efs, WP ef @ s; ⊤ {{ _, True }})
+    ⊢ WP e1 @ s; E {{ Φ }}.
   Proof using Hinh.
     iIntros (???) "H"; iApply wp_lift_pure_det_step; eauto.
-    by destruct p; eauto.
+    by destruct s; eauto.
   Qed.
 
-  Lemma ownP_lift_pure_det_head_step_no_fork {p E Φ} e1 e2 :
+  Lemma ownP_lift_pure_det_head_step_no_fork {s E Φ} e1 e2 :
     to_val e1 = None →
     (∀ σ1, head_reducible e1 σ1) →
     (∀ σ1 e2' σ2 efs', head_step e1 σ1 e2' σ2 efs' → σ1 = σ2 ∧ e2 = e2' ∧ [] = efs') →
-    ▷ WP e2 @ p; E {{ Φ }} ⊢ WP e1 @ p; E {{ Φ }}.
+    ▷ WP e2 @ s; E {{ Φ }} ⊢ WP e1 @ s; E {{ Φ }}.
   Proof using Hinh.
     iIntros (???) "H". iApply ownP_lift_pure_det_step_no_fork; eauto.
-    by destruct p; eauto.
+    by destruct s; eauto.
   Qed.
 End ectx_lifting.
